---
aliases: 
title: Homework 4
---


| **Course**        | Introduction to Robotics |
| ----------------- | ------------------------ |
| **Course Number** | 00350001                 |

| סטודנט א'                      | סטודנט ב'                      | סטודנט ג'                        |
| ------------------------------ | ------------------------------ | -------------------------------- |
| עידו פנג בנטוב                 | ניר קרל                        | אופיר רובין                      |
| 322869140                      | 322437203                      | 211544275                        |
| ido.fang@campus.technion.ac.il | nir.karl@campus.technion.ac.il | ofir.rubin@campus.technion.ac.il |


<div><hr><hr></div>

## Question 1

We are given:

![[IRB1_HW004 תרגיל בית 4 2025-06-08 17.29.08.excalidraw.svg]]^figure-q1a-frames
>Given manipulator.

$$\begin{aligned}
 & ^{0}\mathbf{T}_{1}=\begin{pmatrix}
{c}_{1} & -{s}_{1} & 0 & {\ell}_{1}{c}_{1} \\
{s}_{1} & {c}_{1} & 0 & {\ell}_{1}{s}_{1} \\
0 & 0 & 1 & {h}_{1} \\
0 & 0 & 0 & 1
\end{pmatrix},  & & ^{1}\mathbf{T}_{2}=\begin{pmatrix}
{c}_{2} & 0 & {s}_{2} & 0 \\
{s}_{2} & 0 & -{c}_{2} & 0 \\
0 & 1 & 0 & {h}_{2} \\
0 & 0 & 0 & 1
\end{pmatrix} \\[3ex]
 & ^{2}\mathbf{T}_{3}=\begin{pmatrix}
{c}_{3} & -{s}_{3} & 0 & {\ell}_{3}{c}_{3} \\
{s}_{3} & {c}_{3} & 0 & {\ell}_{3}{s}_{3} \\
0 & 0 & 1 & 0 \\
0 & 0 & 0 & 1
\end{pmatrix}
\end{aligned}$$

Therefore the world to frame transformations:
$$\begin{aligned}
\\[1ex]
 & ^{0}\mathbf{T}_{2}=\begin{pmatrix}
{c}_{12} & 0 & {s}_{12} & {\ell}_{1}{c}_{1} \\
{s}_{12} & 0 & -{c}_{12} & {\ell}_{1}{s}_{1} \\
0 & 1 & 0 & {h}_{1}+{h}_{2} \\
0 & 0 & 0 & 1
\end{pmatrix} \\[2ex]
 & ^{0}\mathbf{T}_{3}=\begin{pmatrix}
{c}_{12}{c}_{3} & -{c}_{12}{s}_{3} & {s}_{12} & {\ell}_{1}{c}_{1}+{\ell}_{3}{c}_{12}{c}_{3} \\
{s}_{12}{c}_{3} & -{s}_{12}{s}_{3} & -{c}_{12} & {\ell}_{1}{s}_{1}+{\ell}_{3}{s}_{12}{c}_{3} \\
{s}_{3} & {c}_{3} & 0 & {h}_{1}+{h}_{2}+{\ell}_{3}{s}_{3} \\
0 & 0 & 0 & 1
\end{pmatrix}
\end{aligned}$$

### Part a
To compute the Jacobian matrix, we'll first follow the [[IRB1_004 Velocity Kinematics and Statics#Systematic Algorithm for Computing the Jacobian|systematic algorithm]], and as an alternative we'll look at the [[IRB1_004 Velocity Kinematics and Statics#Linear Jacobian Computation - Shortcut|shortcut]].

**Systematic Algorithm**:
From the transformation matrices, we extract:

For frame $0$:
$$\mathbf{z}_{0}=\begin{pmatrix}
0 \\
0 \\
1
\end{pmatrix},\qquad \mathbf{p}_{0}=\begin{pmatrix}
0 \\
0 \\
0
\end{pmatrix}$$
For frame $1$:
$$\mathbf{z}_{1}=\begin{pmatrix}
0 \\
0 \\
1
\end{pmatrix},\qquad \mathbf{p}_{1}=\begin{pmatrix}
{\ell}_{1}{c}_{1} \\
{\ell}_{1}{s}_{1} \\
{h}_{1}
\end{pmatrix}$$
For frame $2$:
$$\mathbf{z}_{2}=\begin{pmatrix}
{s}_{12} \\
-{c}_{12} \\
0
\end{pmatrix},\qquad \mathbf{p}_{2}=\begin{pmatrix}
{\ell}_{1}{c}_{1} \\
{\ell}_{1}{s}_{1} \\
{h}_{1}+{h}_{2}
\end{pmatrix}
$$
For frame $3$:
$$\mathbf{z}_{3}=\begin{pmatrix}
{s}_{12} \\
-{c}_{12} \\
0
\end{pmatrix},\qquad \mathbf{p}_{3}=\begin{pmatrix}
{\ell}_{1}{c}_{1}+{\ell}_{3}{c}_{12}{c}_{3} \\
{\ell}_{1}{s}_{1}+{\ell}_{3}{s}_{12}{c}_{3} \\
{h}_{1}+{h}_{2}+{\ell}_{3}{s}_{3}
\end{pmatrix}$$

Now to compute the Jacobian columns, for joint $1$ (revolute joint):
$$\begin{aligned}
  \mathbf{J}_{L1} & =
\mathbf{z}_{0}\times(\mathbf{p}_{3}-\mathbf{p}_{0})\\[1ex]
 & =\begin{pmatrix}
0 \\
0 \\
1
\end{pmatrix}\times \begin{pmatrix}
{\ell}_{1}{c}_{1}+{\ell}_{3}{c}_{12}{c}_{3} \\
{\ell}_{1}{s}_{1}+{\ell}_{3}{s}_{12}{c}_{3} \\
{h}_{1}+{h}_{2}+{\ell}_{3}{s}_{3}
\end{pmatrix} \\[1ex]
 & =\begin{pmatrix}
-{\ell}_{1}{s}_{1}-{\ell}_{3}{s}_{12}{c}_{3} \\
{\ell}_{1}{c}_{1}+{\ell}_{3}{c}_{12}{c}_{3} \\
0
\end{pmatrix} \\[3ex]
\mathbf{J}_{A 1}   & =\mathbf{z}_{0} =\begin{pmatrix}
0 \\
0 \\
1
\end{pmatrix}
\end{aligned}$$

For joint $2$ (revolute joint):
$$\begin{aligned}
\mathbf{J}_{L2} & =
\mathbf{z}_{1}\times(\mathbf{p}_{3}-\mathbf{p}_{1})\\[1ex]
 & =\begin{pmatrix}
0 \\
0 \\
1
\end{pmatrix}\times \begin{pmatrix}
{\ell}_{3}{c}_{12}{c}_{3} \\
{\ell}_{3}{s}_{12}{c}_{3} \\
{h}_{2}+{\ell}_{3}{s}_{3}
\end{pmatrix} \\[1ex]
 & =\begin{pmatrix}
-{\ell}_{3}{s}_{12}{c}_{3} \\
{\ell}_{3}{c}_{12}{c}_{3} \\
0
\end{pmatrix} \\[3ex]
\mathbf{J}_{A 2}   & =\mathbf{z}_{1} =\begin{pmatrix}
0 \\
0 \\
1
\end{pmatrix}
\end{aligned}$$

For joint $3$ (revolute joint):
$$\begin{aligned}
\mathbf{J}_{L3}  & ={\mathbf{z}}_{2}\times (\mathbf{p}_{3}-\mathbf{p}_{2}) \\[1ex]
 & =\begin{pmatrix}
{s}_{12} \\
-{c}_{12} \\
0
\end{pmatrix}\times \begin{pmatrix}
{\ell}_{3}{c}_{12}{c}_{3} \\
{\ell}_{3}{s}_{12}{c}_{3} \\
{\ell}_{3}{s}_{3}
\end{pmatrix} \\[1ex]
 & =\begin{pmatrix}
-{c}_{12}{\ell}_{3}{s}_{3} \\
-{s}_{12}{\ell}_{3}{s}_{3} \\
{\ell}_{3}{c}_{3}
\end{pmatrix} \\[3ex]
\mathbf{J}_{A 3} & =\mathbf{z}_{2}=\begin{pmatrix}
{s}_{12} \\
-{c}_{12} \\
0
\end{pmatrix}
\end{aligned}$$

Therefore:
$$\boxed {
\mathbf{J}_{}=\begin{pmatrix}
-{\ell}_{1}{s}_{1}-{\ell}_{3}{s}_{12}{c}_{3}  & -{\ell}_{3}{s}_{12}{c}_{3} & -{c}_{12}{\ell}_{3}{s}_{3} \\
{\ell}_{1}{c}_{1}+{\ell}_{3}{c}_{12}{c}_{3}  & {\ell}_{3}{c}_{12}{c}_{3}  & -{s}_{12}{\ell}_{3}{s}_{3}\\
0 & 0 & {\ell}_{3}{c}_{3} \\
0  & 0  & {s}_{12} \\
0  & 0 & -{c}_{12}\\
1 & 1 & 0
\end{pmatrix}
 }$$

 
**Shortcut**:
From the forward kinematics, the end-effector position is:
$$\mathbf{p}_3 = \begin{pmatrix}
{\ell}_{1}{c}_{1}+{\ell}_{3}{c}_{12}{c}_{3} \\
{\ell}_{1}{s}_{1}+{\ell}_{3}{s}_{12}{c}_{3} \\
{h}_{1}+{h}_{2}+{\ell}_{3}{s}_{3}
\end{pmatrix}$$

We can compute the linear Jacobian by direct differentiation:
$$\mathbf{J}_{L}=\dfrac{ \partial \mathbf{p}_{3} }{ \partial {\boldsymbol{\theta}} }= \begin{pmatrix}
-{\ell}_{1}{s}_{1}-{\ell}_{3}{s}_{12}{c}_{3} & -{\ell}_{3}{s}_{12}{c}_{3} & -{\ell}_{3}{c}_{12}{s}_{3} \\[1ex]
{\ell}_{1}{c}_{1}+{\ell}_{3}{c}_{12}{c}_{3} & {\ell}_{3}{c}_{12}{c}_{3} & -{\ell}_{3}{s}_{12}{s}_{3} \\
0 & 0 & {\ell}_{3}{c}_{3}
\end{pmatrix} $$


### Part b
The joint values at which the manipulator configuration is singular are where $\det(\mathbf{J}_{L})=0$. That is:
$$\begin{aligned}
\det(\mathbf{J}_{L}) & ={\ell}_{3}{c}_{3}\begin{vmatrix}
-{\ell}_{1}{s}_{1}-{\ell}_{3}{s}_{12}{c}_{3} & -{\ell}_{3}{s}_{12}{c}_{3} \\
{\ell}_{1}{c}_{1}+{\ell}_{3}{c}_{12}{c}_{3} & {\ell}_{3}{c}_{12}{c}_{3}
\end{vmatrix} \\[1ex]
 & ={\ell}_{3}{c}_{3}\left[(-{\ell}_{1}{s}_{1}-{\ell}_{3}{s}_{12}{c}_{3})({\ell}_{3}{c}_{12}{c}_{3}) - (-{\ell}_{3}{s}_{12}{c}_{3})({\ell}_{1}{c}_{1}+{\ell}_{3}{c}_{12}{c}_{3})\right] \\[1ex]
 & ={\ell}_{3}{c}_{3}\left[-{\ell}_{1}{\ell}_{3}{s}_{1}{c}_{12}{c}_{3} - {{{\ell}_{3}}}^{2}{s}_{12}{c}_{12}{{{c}_{3}}}^{2} + {\ell}_{3}{s}_{12}{c}_{3}{\ell}_{1}{c}_{1} + {{{\ell}_{3}}}^{2}{s}_{12}{c}_{12}{{{c}_{3}}}^{2}\right] \\[1ex]
 & ={\ell}_{3}{c}_{3}\left[{\ell}_{1}{\ell}_{3}{c}_{3}(-{s}_{1}{c}_{12} + {s}_{12}{c}_{1})\right] \\[1ex]
 & ={\ell}_{1}{{{\ell}_{3}}}^{2}{{{c}_{3}}}^{2}\sin({\theta}_{1}+{\theta}_{2}-{\theta}_{1}) \\[1ex]
 & ={\ell}_{1}{{{\ell}_{3}}}^{2}{{{c}_{3}}}^{2}{s}_{2}
\end{aligned}$$

Therefore, the manipulator is singular when:
$$\boxed{\theta_2 = 0, \pi \quad \text{or} \quad \theta_3 = \pm\frac{\pi}{2}}$$

These correspond to:
1. $\theta_2 = 0, \pi$: The second and third joints are collinear
2. $\theta_3 = \pm\frac{\pi}{2}$: The end-effector is at maximum/minimum reach in the $z$-direction

![[IRB1_HW004 תרגיל בית 4 2025-06-10 21.33.22.excalidraw.svg]]^figure-q1-singular
>(Left) Singular configuration where ${\theta}_{2}=0$. (Right) Singular configuration where ${\theta}_{3}=\pi /2$.

### Part c
The new manipulator will be of the form:
![[IRB1_HW004 תרגיל בית 4 2025-06-10 22.00.38.excalidraw.svg]]^figure-q1c-fixed
>RR manipulator with $\theta_2 = 0$ fixed.

For the RR manipulator with $\theta_2 = 0$ fixed, we have $s_2 = 0$ and $c_2 = 1$, so $s_{12} = s_1$ and $c_{12} = c_1$.

The end-effector position becomes:
$$\mathbf{p}_3 = \begin{pmatrix}
{\ell}_{1}{c}_{1} + {\ell}_{3}{c}_{1}{c}_{3} \\
{\ell}_{1}{s}_{1} + {\ell}_{3}{s}_{1}{c}_{3} \\
{h}_{1} + {h}_{2} + {\ell}_{3}{s}_{3}
\end{pmatrix}$$

The Jacobian matrix for this RR manipulator is:
$$\mathbf{J}_{L} = \frac{\partial \mathbf{p}_3}{\partial [\theta_1, \theta_3]} = \begin{pmatrix}
-{s}_{1}({\ell}_{1} + {\ell}_{3}{c}_{3}) & -{\ell}_{3}{c}_{1}{s}_{3} \\
{c}_{1}({\ell}_{1} + {\ell}_{3}{c}_{3}) & -{\ell}_{3}{s}_{1}{s}_{3} \\
0 & {\ell}_{3}{c}_{3}
\end{pmatrix}$$

This is a $3 \times 2$ matrix. For the manipulator to be non-singular, this matrix must have full rank (rank = $2$).

**Singularity Analysis:**
The rank is less than $2$ when all $2 \times 2$ minors are zero. The possible minors are:

**Minor from rows (1,2):**
$$M_{12} = \begin{vmatrix}
-{s}_{1}({\ell}_{1} + {\ell}_{3}{c}_{3}) & -{\ell}_{3}{c}_{1}{s}_{3} \\
{c}_{1}({\ell}_{1} + {\ell}_{3}{c}_{3}) & -{\ell}_{3}{s}_{1}{s}_{3}
\end{vmatrix} = {\ell}_{3}{s}_{3}({\ell}_{1} + {\ell}_{3}{c}_{3})$$

**Minor from rows (1,3):**
$$M_{13} = \begin{vmatrix}
-{s}_{1}({\ell}_{1} + {\ell}_{3}{c}_{3}) & -{\ell}_{3}{c}_{1}{s}_{3} \\
0 & {\ell}_{3}{c}_{3}
\end{vmatrix} = -{\ell}_{3}{c}_{3}{s}_{1}({\ell}_{1} + {\ell}_{3}{c}_{3})$$

**Minor from rows (2,3):**
$$M_{23} = \begin{vmatrix}
{c}_{1}({\ell}_{1} + {\ell}_{3}{c}_{3}) & -{\ell}_{3}{s}_{1}{s}_{3} \\
0 & {\ell}_{3}{c}_{3}
\end{vmatrix} = {\ell}_{3}{c}_{3}{c}_{1}({\ell}_{1} + {\ell}_{3}{c}_{3})$$

For singularity, ALL minors must be zero simultaneously.

**From $M_{13} = 0$ and $M_{23} = 0$:** 
Both minors contain the factor ${\ell}_{3}{c}_{3}$. Since $\ell_3 \neq 0$, we need ${c}_{3} = 0$ (i.e., $\theta_3 = \pm\pi /2$).

Since $M_{12} \neq 0$ when $c_3 = 0$, **not all minors are zero**, so $\theta_3 = \pm \pi /2$ is **NOT** a singularity.

**From $M_{12} = 0$:**
$$M_{12} = {\ell}_{3}{s}_{3}({\ell}_{1} + {\ell}_{3}{c}_{3}) = 0$$

This requires either:
1. $s_3 = 0$ (i.e., $\theta_3 = 0, \pi$), or  
2. ${\ell}_{1} + {\ell}_{3}{c}_{3} = 0$

**Case 1: $\theta_3 = 0, \pi$ ($s_3 = 0$)**
- When $\theta_3 = 0$: $c_3 = 1$, so:
  - $M_{13} = -{\ell}_{3}{s}_{1}({\ell}_{1} + {\ell}_{3}) \neq 0$ (unless $s_1 = 0$)
  - $M_{23} = {\ell}_{3}{c}_{1}({\ell}_{1} + {\ell}_{3}) \neq 0$ (unless $c_1 = 0$)
  
  Since $s_1$ and $c_1$ cannot both be zero, at least one of $M_{13}$ or $M_{23}$ is non-zero.

- When $\theta_3 = \pi$: $c_3 = -1$, so:
  - $M_{13} = {\ell}_{3}{s}_{1}({\ell}_{1} - {\ell}_{3})$
  - $M_{23} = -{\ell}_{3}{c}_{1}({\ell}_{1} - {\ell}_{3})$

For ALL minors to be zero at $\theta_3 = \pi$, we need both $M_{13} = 0$ and $M_{23} = 0$. Since $s_1$ and $c_1$ cannot both be zero, we need ${\ell}_{1} - {\ell}_{3} = 0$, i.e., ${\ell}_{1} = {\ell}_{3}$.

**Case 2: ${\ell}_{1} + {\ell}_{3}{c}_{3} = 0$**
This gives $c_3 = -{\ell}_{1}/{\ell}_{3}$. For this to be valid, we need $|{\ell}_{1}/{\ell}_{3}| \leq 1$.

**Singularity Condition:**
The RR manipulator is singular when:
$$\boxed{\cos{\theta}_{3} = -\frac{{\ell}_{1}}{{\ell}_{3}} \text{ (provided }{\ell}_{1} \leq {\ell}_{3} \text{)}}$$

This includes the special case $\theta_3 = \pi$ when ${\ell}_{1} = {\ell}_{3}$.

# Question 2
We are given:

![[IRB1_HW004 תרגיל בית 4 2025-06-11 09.14.17.excalidraw.svg]]^figure-q2-frames
>Given manipulator.

$$^{0}\mathbf{T}_{3}=\begin{pmatrix}
{c}_{13} & -{s}_{13} & 0 & {\ell}_{1}{c}_{1}-{d}_{2}{s}_{1}+{\ell}_{3}{c}_{13} \\
{s}_{13} & {c}_{13} & 0 & {\ell}_{1}{s}_{1}+{d}_{2}{c}_{1}+{\ell}_{3}{s}_{13} \\
0  & 0 & 1 & 0 \\
0 & 0 & 0 &  1
\end{pmatrix}$$

### Part a
The linear Jacobian would be:
$$\mathbf{J}_{L}=\dfrac{ \partial \mathbf{p}_{3} }{ \partial \boldsymbol{\theta} }=\begin{pmatrix}
-{\ell}_{1}{s}_{1}-{d}_{2}{c}_{1}-{\ell}_{3}{s}_{13} & -{s}_{1} & -{\ell}_{3}{s}_{13} \\
{\ell}_{1}{c}_{1}-{d}_{2}{s}_{1}+{\ell}_{3}{c}_{13} & {c}_{1} & {\ell}_{3}{c}_{13} \\
0 & 0 & 0
\end{pmatrix} $$
Therefore the whole Jacobian:
$$\boxed {
\mathbf{J}=\begin{pmatrix}
-{\ell}_{1}{s}_{1}-{d}_{2}{c}_{1}-{\ell}_{3}{s}_{13} & -{s}_{1} & -{\ell}_{3}{s}_{13} \\
{\ell}_{1}{c}_{1}-{d}_{2}{s}_{1}+{\ell}_{3}{c}_{13} & {c}_{1} & {\ell}_{3}{c}_{13} \\
0 & 0 & 0 \\
0 & 0 & 0 \\
0  & 0 & 0\\
1 & 0 & 1
\end{pmatrix}
 } $$
Where $\mathbf{J}_{A1}=\mathbf{J}_{A 3}=\begin{pmatrix}0 & 0 & 1\end{pmatrix}^{T}$ since this is a planar manipulator.

### Part b
The joint values at which the manipulator configuration is singular are where the linear Jacobian loses rank. Since this is a planar manipulator with 3 DOF but only 2 spatial dimensions, we need to check when all $2\times 2$ minors of $\mathbf{J}_{L}$ become zero.

The three possible $2\times 2$ minors are:

**Minor from columns (1,2):**
$$\begin{aligned}
M_{12} &= \begin{vmatrix}
-{\ell}_{1}{s}_{1}-{d}_{2}{c}_{1}-{\ell}_{3}{s}_{13} & -{s}_{1} \\
{\ell}_{1}{c}_{1}-{d}_{2}{s}_{1}+{\ell}_{3}{c}_{13} & {c}_{1}
\end{vmatrix} \\[1ex]
&= (-{\ell}_{1}{s}_{1}-{d}_{2}{c}_{1}-{\ell}_{3}{s}_{13}){c}_{1} - (-{s}_{1})({\ell}_{1}{c}_{1}-{d}_{2}{s}_{1}+{\ell}_{3}{c}_{13}) \\[1ex]
&= -{\ell}_{1}{s}_{1}{c}_{1}-{d}_{2}{c}_{1}^{2}-{\ell}_{3}{s}_{13}{c}_{1} + {s}_{1}{\ell}_{1}{c}_{1} - {d}_{2}{s}_{1}^{2} + {\ell}_{3}{s}_{1}{c}_{13} \\[1ex]
&= -{d}_{2} - {\ell}_{3}{s}_{13}{c}_{1} + {\ell}_{3}{s}_{1}{c}_{13}  \\[1ex]
 & = -{d}_{2} - {\ell}_{3}{s}_{3}
\end{aligned}$$

**Minor from columns (1,3):**
$$\begin{aligned}
M_{13} &= \begin{vmatrix}
-{\ell}_{1}{s}_{1}-{d}_{2}{c}_{1}-{\ell}_{3}{s}_{13} & -{\ell}_{3}{s}_{13} \\
{\ell}_{1}{c}_{1}-{d}_{2}{s}_{1}+{\ell}_{3}{c}_{13} & {\ell}_{3}{c}_{13}
\end{vmatrix} \\[1ex]
&= (-{\ell}_{1}{s}_{1}-{d}_{2}{c}_{1}-{\ell}_{3}{s}_{13})({\ell}_{3}{c}_{13}) - (-{\ell}_{3}{s}_{13})({\ell}_{1}{c}_{1}-{d}_{2}{s}_{1}+{\ell}_{3}{c}_{13}) \\[1ex]
&= -{\ell}_{1}{\ell}_{3}{s}_{1}{c}_{13} - {d}_{2}{\ell}_{3}{c}_{1}{c}_{13} - {\ell}_{3}^{2}{s}_{13}{c}_{13} + {\ell}_{3}{s}_{13}({\ell}_{1}{c}_{1}-{d}_{2}{s}_{1}+{\ell}_{3}{c}_{13}) \\[1ex]
&= {\ell}_{3}[{\ell}_{1}({s}_{13}{c}_{1} - {s}_{1}{c}_{13}) + {d}_{2}({s}_{13}{s}_{1} - {c}_{1}{c}_{13})] \\[1ex]
&= {\ell}_{3}[{\ell}_{1}\sin(\theta_{13} - \theta_{1}) + {d}_{2}\sin(\theta_{13} - \theta_{1} - \pi/2)] \\[1ex]
&= {\ell}_{3}[{\ell}_{1}{s}_{3} - {d}_{2}{c}_{3}]
\end{aligned}$$

**Minor from columns (2,3):**
$$\begin{aligned}
M_{23} &= \begin{vmatrix}
-{s}_{1} & -{\ell}_{3}{s}_{13} \\
{c}_{1} & {\ell}_{3}{c}_{13}
\end{vmatrix} \\[1ex]
&= -{s}_{1}{\ell}_{3}{c}_{13} - (-{\ell}_{3}{s}_{13}){c}_{1} \\[1ex]
&= {\ell}_{3}({c}_{1}{s}_{13} - {s}_{1}{c}_{13}) \\[1ex]
&= {\ell}_{3}{s}_{3}
\end{aligned}$$

**Singularity Conditions:**
The manipulator is singular when **any** of these minors equals zero:

1. **From $M_{12} = 0$:** $\sin{\theta}_{3} = -\dfrac{{d}_{2}}{{\ell}_{3}}$
2. **From $M_{13} = 0$:** ${\ell}_{1}{s}_{3} = {d}_{2}{c}_{3}$, which gives $\tan{\theta}_{3} = \dfrac{{d}_{2}}{{\ell}_{1}}$
3. **From $M_{23} = 0$:** $\sin{\theta}_{3} = 0$, which gives $\theta_{3} = 0, \pi$

Therefore, the complete set of singularities is:
$$\boxed{\sin{\theta}_{3} = -\dfrac{{d}_{2}}{{\ell}_{3}} \quad \text{or} \quad \tan{\theta}_{3} = \dfrac{{d}_{2}}{{\ell}_{1}} \quad \text{or} \quad \theta_{3} = 0, \pi}$$

![[IRB1_HW004 תרגיל בית 4 2025-06-11 10.18.01.excalidraw.svg]]^figure-q2-singular
>(Left) Singular configuration where $\sin{\theta}_{3}=-{d}_{2}/{\ell}_{3}$. (Center) Singular configuration where $\tan{\theta}_{3}={d}_{2}/{\ell}_{1}$. (Right) Singular configuration where $\theta_{3}=0$.

### Part c

Given that masses $m_1$ and $m_2$ are located at the middle of their respective links, and mass $m_3$ is held at the gripper's origin, we need to compute the generalized force vector required to maintain static equilibrium under gravity.

**Solution:**

Using the **principle of superposition** from [[IRB1_004 Velocity Kinematics and Statics#Multi-Body Static Analysis|manipulator statics]], we treat each mass separately and sum their contributions:****

$$\boldsymbol{\tau}_{\text{total}} = \boldsymbol{\tau}_{m_1} + \boldsymbol{\tau}_{m_2} + \boldsymbol{\tau}_{m_3}$$

**Determine Mass Positions**

From the transformation matrix and manipulator configuration:

**Mass $m_1$ (middle of link 1):**
Link 1 extends from the base to joint 2 over distance $\ell_1$. The center of mass is at:
$$\mathbf{p}_{m_1} = \begin{pmatrix} \frac{\ell_1}{2} c_1 \\ \frac{\ell_1}{2} s_1 \\ 0 \end{pmatrix}$$

**Mass $m_2$ (middle of link 2):**
Link 2 is the prismatic joint extending distance $d_2$ from joint 1. The center of mass is at:
$$\mathbf{p}_{m_2} = \begin{pmatrix} \ell_1 c_1 - \frac{d_2}{2} s_1 \\ \ell_1 s_1 + \frac{d_2}{2} c_1 \\ 0 \end{pmatrix}$$****

**Mass $m_3$ (at gripper origin):**
From the given transformation matrix:
$$\mathbf{p}_{m_3} = \begin{pmatrix} \ell_1 c_1 - d_2 s_1 + \ell_3 c_{13} \\ \ell_1 s_1 + d_2 c_1 + \ell_3 s_{13} \\ 0 \end{pmatrix}$$

**Compute Jacobians for Each Mass**

**For mass $m_1$:**
Only joint $1$ affects the position of $m_1$:
$$\mathbf{J}_{L,m_1} = \frac{\partial \mathbf{p}_{m_1}}{\partial [\theta_1, d_2, \theta_3]} = \begin{pmatrix} -\frac{\ell_1}{2} s_1 & 0 & 0 \\ \frac{\ell_1}{2} c_1 & 0 & 0 \\ 0 & 0 & 0 \end{pmatrix}$$

**For mass $m_2$:**
Joints $1$ and $2$ affect the position of $m_2$:
$$\mathbf{J}_{L,m_2} = \frac{\partial \mathbf{p}_{m_2}}{\partial [\theta_1, d_2, \theta_3]} = \begin{pmatrix} -\ell_1 s_1 - \frac{d_2}{2} c_1 & -\frac{s_1}{2} & 0 \\ \ell_1 c_1 - \frac{d_2}{2} s_1 & \frac{c_1}{2} & 0 \\ 0 & 0 & 0 \end{pmatrix}$$

**For mass $m_3$:**
We use the full Jacobian from part a (linear part only for planar motion):
$$\mathbf{J}_{L,m_3} = \begin{pmatrix} -\ell_1 s_1 - d_2 c_1 - \ell_3 s_{13} & -s_1 & -\ell_3 s_{13} \\ \ell_1 c_1 - d_2 s_1 + \ell_3 c_{13} & c_1 & \ell_3 c_{13} \\ 0 & 0 & 0 \end{pmatrix}$$

**Apply Gravitational Forces**

Each mass experiences gravitational force:
$$\mathbf{F}_{g,i} = \begin{pmatrix} 0 \\ -m_i g \\ 0 \end{pmatrix}$$

**Compute Joint Torques**

Using $\boldsymbol{\tau}_i = \mathbf{J}_{L,i}^T \mathbf{F}_{g,i}$:

**For mass $m_1$:**
$$\begin{aligned}
\boldsymbol{\tau}_{m_1}  & = \mathbf{J}_{L,m_1}^T \begin{pmatrix} 0 \\ -m_1 g \\ 0 \end{pmatrix}  \\[2ex]
 & = \begin{pmatrix} -\frac{\ell_1}{2} s_1 & \frac{\ell_1}{2} c_1 & 0 \\ 0 & 0 & 0 \\ 0 & 0 & 0 \end{pmatrix} \begin{pmatrix} 0 \\ -m_1 g \\ 0 \end{pmatrix}  \\[2ex]
 & = \begin{pmatrix} -\frac{\ell_1 m_1 g c_1}{2} \\ 0 \\ 0 \end{pmatrix}
\end{aligned}$$

**For mass $m_2$:**
$$\begin{aligned}
\boldsymbol{\tau}_{m_2}  & = \mathbf{J}_{L,m_2}^T \begin{pmatrix} 0 \\ -m_2 g \\ 0 \end{pmatrix}  \\[2ex]
 & = \begin{pmatrix} -\ell_1 s_1 - \frac{d_2}{2} c_1 & \ell_1 c_1 - \frac{d_2}{2} s_1 & 0 \\ -\frac{s_1}{2} & \frac{c_1}{2} & 0 \\ 0 & 0 & 0 \end{pmatrix} \begin{pmatrix} 0 \\ -m_2 g \\ 0 \end{pmatrix} \\[2ex]
 & = \begin{pmatrix} -m_2 g(\ell_1 c_1 - \frac{d_2}{2} s_1) \\ -\frac{m_2 g c_1}{2} \\ 0 \end{pmatrix}
\end{aligned}$$

**For mass $m_3$:**
$$\begin{aligned}
\boldsymbol{\tau}_{m_3}  & = \mathbf{J}_{L,m_3}^T \begin{pmatrix} 0 \\ -m_3 g \\ 0 \end{pmatrix}  \\[2ex]
 & = \begin{pmatrix} -\ell_1 s_1 - d_2 c_1 - \ell_3 s_{13} & \ell_1 c_1 - d_2 s_1 + \ell_3 c_{13} & 0 \\ -s_1 & c_1 & 0 \\ -\ell_3 s_{13} & \ell_3 c_{13} & 0 \end{pmatrix} \begin{pmatrix} 0 \\ -m_3 g \\ 0 \end{pmatrix} \\[2ex]
 & = \begin{pmatrix} -m_3 g(\ell_1 c_1 - d_2 s_1 + \ell_3 c_{13}) \\ -m_3 g c_1 \\ -m_3 g \ell_3 c_{13} \end{pmatrix}
\end{aligned}$$


**Total Generalized Forces**

Summing all contributions:
$$\boldsymbol{\tau}_{\text{total}} = \boldsymbol{\tau}_{m_1} + \boldsymbol{\tau}_{m_2} + \boldsymbol{\tau}_{m_3}$$
For each joint:
$$\begin{aligned}
\tau_1 &= -\frac{\ell_1 m_1 g c_1}{2} - m_2 g(\ell_1 c_1 - \frac{d_2}{2} s_1) - m_3 g(\ell_1 c_1 - d_2 s_1 + \ell_3 c_{13}) \\[1ex]
&= -g c_1 \left(\frac{\ell_1 m_1}{2} + m_2 \ell_1 + m_3 \ell_1\right) + g s_1 \left(\frac{m_2 d_2}{2} + m_3 d_2\right) - m_3 g \ell_3 c_{13} \\[2ex]
\tau_2 &= -\frac{m_2 g c_1}{2} - m_3 g c_1 = -g c_1 \left(\frac{m_2}{2} + m_3\right) \\[2ex]
\tau_3 &= -m_3 g \ell_3 c_{13}
\end{aligned}$$

The generalized forces that gravity applies to the system are:
$$\boldsymbol{\tau}_{\text{gravity}} = \small\begin{pmatrix} 
-g c_1 \left(\frac{\ell_1 m_1}{2} + m_2 \ell_1 + m_3 \ell_1\right) + g s_1 \left(\frac{m_2 d_2}{2} + m_3 d_2\right) - m_3 g \ell_3 c_{13} \\[1ex]
-g c_1 \left(\frac{m_2}{2} + m_3\right) \\[1ex]
-m_3 g \ell_3 c_{13}
\end{pmatrix}$$

Therefore, the generalized force vector that the **joints must apply** to maintain static equilibrium is $\tau \mathbf{_{\text{joints}}}=-\boldsymbol{\tau}_{\text{gravity}}$:

$$\boxed{\boldsymbol{\tau}_{\text{joints}}  = \small\begin{pmatrix} 
g c_1 \left(\frac{\ell_1 m_1}{2} + m_2 \ell_1 + m_3 \ell_1\right) - g s_1 \left(\frac{m_2 d_2}{2} + m_3 d_2\right) + m_3 g \ell_3 c_{13} \\[1ex]
g c_1 \left(\frac{m_2}{2} + m_3\right) \\[1ex]
m_3 g \ell_3 c_{13}
\end{pmatrix}}$$
