---
aliases:
---
## Question 1
We are given the following:
![[IRB1_HW006 תרגיל בית 6 2025-07-04 13.58.34.excalidraw.svg]]


with the following D–H Parameters:
$$\begin{array}{c|cccc}
i & \alpha _{i} & {a}_{i} & {d}_{i} & {\theta}_{i} \\
\hline 1    & 270^{\circ}  & 0 & 0 & {\theta}_{1} \\
2 & 0  & 0 &r & 90^{\circ}  \\
\end{array}$$

The transformation matrices are given as:
$$\begin{aligned}
 & {}^0\mathbf{T}_1  = \begin{pmatrix}
c_1 & 0 & -s_1 & 0 \\
s_1 & 0 & c_1 & 0 \\
0 & -1 & 0 & 0 \\
0 & 0 & 0 & 1
\end{pmatrix} \\[2ex]
 & {}^0\mathbf{T}_2 = {}^0\mathbf{T}_1 {}^1\mathbf{T}_2 = \begin{pmatrix}
0 & -{c}_{1} & -s_1 & -r{s}_{1} \\
0 & -{s}_{1} & {c}_{1} & r{c}_{1} \\
0 & 0 & 0 & 0 \\
0 & 0 & 0 & 1
\end{pmatrix}
\end{aligned}$$

### Part a
**Generalized Coordinates**
For this RP manipulator: $\mathbf{q} = [\theta_1, r]^T$ where:
- $\theta_1$ is the revolute joint angle
- $r$ is the prismatic joint extension

**Position Analysis**
From the given transformation matrices, the key positions are:

End-effector position:
$$\mathbf{p}_{\text{end}} = \begin{pmatrix} -r \sin \theta_1 \\ r \cos \theta_1 \\ 0 \end{pmatrix}$$

Center of mass of link (at distance $r/2$ from base):
$$\mathbf{p}_{\text{cm}} = \begin{pmatrix} -\frac{r}{2} \sin \theta_1 \\ \frac{r}{2} \cos \theta_1 \\ 0 \end{pmatrix}$$

**Velocity Analysis**
Taking time derivatives:

End-effector velocity:
$$\dot{\mathbf{p}}_{\text{end}} = \begin{pmatrix} -\dot{r} \sin \theta_1 - r \cos \theta_1 \dot{\theta}_1 \\ \dot{r} \cos \theta_1 - r \sin \theta_1 \dot{\theta}_1 \\ 0 \end{pmatrix}$$

Center of mass velocity:
$$\dot{\mathbf{p}}_{\text{cm}} = \begin{pmatrix} -\frac{\dot{r}}{2} \sin \theta_1 - \frac{r}{2} \cos \theta_1 \dot{\theta}_1 \\ \frac{\dot{r}}{2} \cos \theta_1 - \frac{r}{2} \sin \theta_1 \dot{\theta}_1 \\ 0 \end{pmatrix}$$

**Kinetic Energy Calculation**:
Translational kinetic energy of the distributed link:
$$\begin{gathered}
|\dot{\mathbf{p}}_{\text{cm}}|^2= \left(\frac{\dot{r}}{2}\right)^2 + \left(\frac{r \dot{\theta}_1}{2}\right)^2 \\[2ex]
\begin{aligned}
\implies T_{\text{link,trans}}  & = \frac{1}{2}M|\dot{\mathbf{p}}_{\text{cm}}|^2  \\[1ex]
 & = \frac{M}{8}(\dot{r}^2 + r^2{{\dot{\theta}_{1}}}^{2})
\end{aligned}
\end{gathered}$$

Rotational kinetic energy of the link:
$$\begin{aligned}
T_{\text{link,rot}}  & = \frac{1}{2}I_c{{\dot{\theta}_{1}}}^{2}  \\[1ex]
 & = \frac{1}{2} \cdot \frac{Mr^2}{12} \cdot {{\dot{\theta}_{1}}}^{2}  \\[1ex]
 & = \frac{Mr^2{{\dot{\theta}_{1}}}^{2}}{24}
\end{aligned}$$

Kinetic energy of point mass:
$$\begin{gathered}
|\dot{\mathbf{p}}_{\text{end}}|^2 = \dot{r}^2 + r^2{{\dot{\theta}_{1}}}^{2} \\[2ex]
\begin{aligned}
\implies T_{\text{mass}}  & = \frac{1}{2}m|\dot{\mathbf{p}}_{\text{end}}|^2  \\[1ex]
 & = \frac{m}{2}(\dot{r}^2 + r^2{{\dot{\theta}_{1}}}^{2})
\end{aligned}
\end{gathered}$$

**Total kinetic energy:**
$$\begin{aligned}
T &= T_{\text{link,trans}} + T_{\text{link,rot}} + T_{\text{mass}} \\[1ex]
&= \frac{M}{8}(\dot{r}^2 + r^2{{\dot{\theta}_{1}}}^{2}) + \frac{Mr^2{{\dot{\theta}_{1}}}^{2}}{24} + \frac{m}{2}(\dot{r}^2 + r^2{{\dot{\theta}_{1}}}^{2}) \\[1ex]
&= \left(\frac{M}{8} + \frac{m}{2}\right)\dot{r}^2 + \left(\frac{M}{8} + \frac{M}{24} + \frac{m}{2}\right)r^2{{\dot{\theta}_{1}}}^{2} \\[1ex]
&= \left(\frac{M + 4m}{8}\right)\dot{r}^2 + \left(\frac{M + 3m}{6}\right)r^2{{\dot{\theta}_{1}}}^{2}
\end{aligned}$$

**Potential Energy**
Since gravity acts along the $z_0$ axis and all motion occurs in the $x$-$y$ plane (as evident from the transformation matrices), there is no change in gravitational potential energy:
$$V = \text{constant} = 0$$

**Lagrangian and Equations of Motion**
The Lagrangian is: $L = T - V = T$

Applying the Euler-Lagrange equations from [[IRB1_005 Dynamics of Open Chains#Basic Concepts|Equation]] $\text{(LP8.3)}$:

**For $\theta_1$**:
$$\begin{aligned}
 & \frac{\partial L}{\partial \dot{\theta}_1} = \frac{M + 3m}{3}r^2\dot{\theta}_1 \\[1ex]
 & \frac{\mathrm{d}}{\mathrm{d}t}\left(\frac{\partial L}{\partial \dot{\theta}_1}\right) = \frac{M + 3m}{3}r^2\ddot{\theta}_1 + \frac{2(M + 3m)}{3}r\dot{r}\dot{\theta}_1 \\[1ex]
 & \frac{\partial L}{\partial \theta_1} = 0
\end{aligned}$$

**For $r$**:
$$\begin{aligned}
 & \frac{\partial L}{\partial \dot{r}} = \frac{M + 4m}{4}\dot{r} \\[1ex]
 & \frac{\mathrm{d}}{\mathrm{d}t}\left(\frac{\partial L}{\partial \dot{r}}\right) = \frac{M + 4m}{4}\ddot{r} \\[1ex]
 & \frac{\partial L}{\partial r} = \frac{M + 3m}{3}r{{\dot{\theta}_{1}}}^{2}
\end{aligned}$$

**Final Matrix Form**
Following the standard form from [[IRB1_005 Dynamics of Open Chains|Equation]] $\text{(LP8.10)}$:

$$\boldsymbol{\tau} = \mathbf{M}(\mathbf{q})\ddot{\mathbf{q}} + \mathbf{C}(\mathbf{q},\dot{\mathbf{q}})\dot{\mathbf{q}} + \mathbf{G}(\mathbf{q})$$
We get:
$$\boxed{ \begin{pmatrix}
{T}_{\theta} \\
  f_r
  \end{pmatrix}=\small\begin{pmatrix}
\frac{M + 3m}{3}r^2 & 0 \\
0 & \frac{M + 4m}{4}
\end{pmatrix} \begin{pmatrix}
\ddot{\theta}_1 \\
\ddot{r}
\end{pmatrix} + \begin{pmatrix}
0 & \frac{2(M + 3m)}{3}r \\[1ex]
-\frac{M + 3m}{3}r & 0
\end{pmatrix} \begin{pmatrix}
\dot{\theta}_1 \\
\dot{r}
\end{pmatrix} + \begin{pmatrix}
0 \\[1ex]
0
\end{pmatrix}}$$
### Part b
We are given:
$$\mathbf{p}(t) = \mathbf{p}_0 + \lambda(t)(\mathbf{p}_f - \mathbf{p}_0), \quad t \in [0,T]$$

where $\lambda(0) = 0$, $\lambda(T) = 1$, $\mathbf{p}_0, \mathbf{p}_f \in \mathbb{R}^k$ are the starting and ending points respectively, $k$ is the dimension of the Euclidean space, and $\lambda(t)$ is a polynomial of degree $n$:

$$\lambda(t) = a_0 + a_1\left(\frac{t}{T}\right) + a_2\left(\frac{t}{T}\right)^2 + \cdots + a_n\left(\frac{t}{T}\right)^n$$

**a. Determine $k$ and $n$**
For this RP manipulator, from the transformation matrices we see that the gripper moves in the $x$-$y$ plane:

$$\boxed{k = 2}$$

For the gripper's motion to begin and end with zero velocity and acceleration, we have the following constraints:

Position constraints:
- $\lambda(0) = 0$ 
- $\lambda(T) = 1$

Velocity constraints:
- $\dot{\lambda}(0) = 0$ (zero initial velocity)
- $\dot{\lambda}(T) = 0$ (zero final velocity)

Acceleration constraints:
- $\ddot{\lambda}(0) = 0$ (zero initial acceleration)
- $\ddot{\lambda}(T) = 0$ (zero final acceleration)

With $c = 6$ total constraints, we need a polynomial of degree:

$$\boxed{n = c - 1 = 5}$$

**b. Compute coefficients $a_0, \ldots, a_n$**
The polynomial is:
$$\lambda(s) = a_0 + a_1 s + a_2 s^2 + a_3 s^3 + a_4 s^4 + a_5 s^5$$

where $s = t/T$. The derivatives are:
$$\begin{aligned}
\dot{\lambda}(s) &= \frac{1}{T}(a_1 + 2a_2 s + 3a_3 s^2 + 4a_4 s^3 + 5a_5 s^4) \\[1ex]
\ddot{\lambda}(s) &= \frac{1}{T^2}(2a_2 + 6a_3 s + 12a_4 s^2 + 20a_5 s^3)
\end{aligned}$$

Applying constraints:
From $\lambda(0)=0$, $\dot{\lambda}(0)=0$, and $\ddot{\lambda}(0)=0$, we get:
$$\boxed{{a}_{0}={a}_{1}={a}_{2}=0 }$$

From $\lambda(1) = 1$, $\dot{\lambda}(1) = 0$, and $\ddot{\lambda}(1) = 0$:
$$\begin{aligned}
 & a_3 + a_4 + a_5 = 1 \\[1ex]
 & 3a_3 + 4a_4 + 5a_5 = 0 \\[1ex]
 & 6a_3 + 12a_4 + 20a_5 = 0
\end{aligned}$$

Solving: $\boxed{a_3 = 10, \quad a_4 = -15, \quad a_5 = 6}$

Final polynomial:
$$\boxed{\lambda(t) = 10\left(\frac{t}{T}\right)^3 - 15\left(\frac{t}{T}\right)^4 + 6\left(\frac{t}{T}\right)^5}$$

**c. Expressions for $\mathbf{p}(t)$, $\dot{\mathbf{p}}(t)$, and $\ddot{\mathbf{p}}(t)$**
Position:
$$\boxed{\mathbf{p}(t) = \mathbf{p}_0 + \lambda(t)(\mathbf{p}_f - \mathbf{p}_0)}$$

  Velocity:
  $$\boxed{\dot{\mathbf{p}}(t) = \dot{\lambda}(t)(\mathbf{p}_f - \mathbf{p}_0)}$$
  
  Acceleration:
  $$\boxed{\ddot{\mathbf{p}}(t) = \ddot{\lambda}(t)(\mathbf{p}_f - \mathbf{p}_0)}$$

where:
$$\begin{aligned}
\dot{\lambda}(t) &= \frac{30}{T}\left(\frac{t}{T}\right)^2\left[1 - 2\left(\frac{t}{T}\right) + \left(\frac{t}{T}\right)^2\right] \\[1ex]
\ddot{\lambda}(t) &= \frac{60}{T^2}\left(\frac{t}{T}\right)\left[1 - 3\left(\frac{t}{T}\right) + 2\left(\frac{t}{T}\right)^2\right]
\end{aligned}$$

**d. Joint values, velocities, and accelerations**
From the position analysis, the gripper position is:
$$\mathbf{p}(t) = \begin{pmatrix} x(t) \\ y(t) \end{pmatrix} = \begin{pmatrix} -r(t) \sin \theta_1(t) \\ r(t) \cos \theta_1(t) \end{pmatrix}$$

Joint values (Inverse Kinematics):
$$\boxed{\begin{aligned}
r(t) &= \sqrt{x^2(t) + y^2(t)} \\[1ex]
\theta_1(t) &= \text{atan2}(-x(t), y(t))
\end{aligned}}$$

Joint velocities:
Using the chain rule and the Jacobian relationship:
$$\boxed{\begin{aligned}
\dot{r}(t) &= \frac{x(t)\dot{x}(t) + y(t)\dot{y}(t)}{\sqrt{x^2(t) + y^2(t)}} \\[1ex]
\dot{\theta}_1(t) &= \frac{-y(t)\dot{x}(t) + x(t)\dot{y}(t)}{x^2(t) + y^2(t)}
\end{aligned}}$$

Joint accelerations:
$$\boxed{\begin{aligned}
\ddot{r}(t) &= \frac{(\dot{x}^2 + \dot{y}^2)r + (x\ddot{x} + y\ddot{y})}{r} - \frac{(x\dot{x} + y\dot{y})^2}{r^3} \\[1ex]
\ddot{\theta}_1(t) &= \frac{(-y\ddot{x} + x\ddot{y})(x^2 + y^2) - (-y\dot{x} + x\dot{y}) \cdot 2(x\dot{x} + y\dot{y})}{(x^2 + y^2)^2}
\end{aligned}}$$

**e. Generalized forces**
Using our solution from [[#Part a]]:

$$\boldsymbol{\tau}(t) = \mathbf{M}(\mathbf{q}(t))\ddot{\mathbf{q}}(t) + \mathbf{C}(\mathbf{q}(t),\dot{\mathbf{q}}(t))\dot{\mathbf{q}}(t)$$

where:
$$\begin{gathered}
\mathbf{M}(\mathbf{q}) = \begin{pmatrix}
\frac{M + 3m}{3}r^2 & 0 \\[1ex]
0 & \frac{M + 4m}{4}
\end{pmatrix} \\[3ex]
\mathbf{C}(\mathbf{q},\dot{\mathbf{q}}) = \begin{pmatrix}
0 & \frac{2(M + 3m)}{3}r \\[1ex]
-\frac{M + 3m}{3}r & 0
\end{pmatrix} \\[3ex]
\mathbf{q}(t) = \begin{pmatrix} \theta_1(t) \\ r(t) \end{pmatrix}, \quad \boldsymbol{\tau}(t) = \begin{pmatrix} T(t) \\ f_r(t) \end{pmatrix}
\end{gathered}$$


Explicitly:
$$\boxed{\begin{aligned}
{T}_{\theta}(t) &= \frac{M + 3m}{3}r^2(t)\ddot{\theta}_1(t) + \frac{2(M + 3m)}{3}r(t)\dot{r}(t)\dot{\theta}_1(t) \\[1ex]
f_r(t) &= \frac{M + 4m}{4}\ddot{r}(t) - \frac{M + 3m}{3}r(t){{\dot{\theta}_{1}}}^{2}(t)
\end{aligned}}$$
